proof/iu_system/decl/properties.v
@@ -3,7 +3,7 @@ Require Import Program.Tactics.
 Require Import Lia.
 Require Import Metalib.Metatheory.
 
-Require Import decl_iu.notations.
+Require Import decl.notations.
 Require Import ln_utils.
 
 Definition wf_dom : forall {Γ}, ⊢ Γ -> atoms.
@@ -143,7 +143,8 @@ Qed.
 
 Theorem ld_wf_type_weakening : 
   forall G1 G2 G3 t, 
-  G1 ,, G3 ⊢ t -> ⊢ G1 ,, G2 ,, G3 -> 
+  G1 ,, G3 ⊢ t -> 
+  ⊢ G1 ,, G2 ,, G3 -> 
   G1 ,, G2 ,, G3 ⊢ t.
 Proof.
   intros.
@@ -152,6 +153,25 @@ Proof.
   - eapply ld_wft_forall with (L:=L `union` ld_ctx_dom (G1,, G2,, G3)). intros.
     inst_cofinites_with x. replace (G1,, G2,, G3, x ) with (G1,, G2,, (G3, x)) by auto. apply H0; auto.
     simpl. econstructor; eauto.
+Qed.
+
+
+Lemma ld_wf_type_fv: forall G t x, 
+  G ⊢ t -> x `notin` ld_ctx_dom G -> x `notin` fv_ld_type t.
+Proof.
+  intros.
+  induction H; simpl in *; auto.
+  - induction G.
+    + inversion H1.
+    + inversion H1; subst.
+      * simpl in H0. auto.
+      * inversion H. simpl in H0. apply IHG; auto.
+  - inst_cofinites_by (L `union` singleton x).
+    assert (x ∉ add x0 (ld_ctx_dom G)) by auto.
+    specialize (H1 H2). 
+    simpl in H1.
+    rewrite fv_ld_type_open_ld_type_wrt_ld_type_lower.
+    eauto.
 Qed.
 
 
@@ -847,5 +867,3 @@ Proof.
   apply ld_sub_to_sized_ld_sub in H0. destruct H0 as [n2].
   eapply generalized_transitivity; eauto.
 Qed.
-
-Print Assumptions transitivity.
