proof/iu_system/transfer.v
@@ -1,0 +1,544 @@
+Require Import Coq.Program.Equality.
+Require Import Program.Tactics.
+Require Import Metalib.Metatheory.
+
+Require Import algo.ott.
+Require Import algo.notations.
+Require Import algo.ln_inf_extra.
+Require Import decl.ott.
+Require Import decl.notations.
+Require Import decl.properties.
+Require Import decl.ln_inf_extra.
+Require Import ln_utils.
+
+
+Inductive ss_entry := 
+  | sse_tv 
+  | sse_ev (t : ld_type).
+
+Definition subst_set := list (var * ss_entry).
+
+Declare Scope subst_set_scope.
+Delimit Scope subst_set_scope with subst.
+Bind Scope subst_set_scope with subst_set.
+
+Notation "s1 ;; s2" := (app s2 s1)
+  (at level 58, left associativity) : subst_set_scope.
+
+Notation "s ; ex : t" := (cons (pair ex (sse_ev t)) s)
+  (at level 58, ex at next level, t at next level, left associativity) : type_scope.
+
+Notation "s ; x" := (cons (pair x sse_tv) s)
+  (at level 58, x at next level, left associativity) : type_scope.
+
+Notation "x : t ∈ s" := (binds x (sse_ev t) s)
+  (at level 58, t at next level, no associativity) : type_scope.
+
+
+Fixpoint fv_ss (θ : subst_set) : atoms :=
+  match θ with
+  | nil => {}
+  | θ' ; ex : t => fv_ss θ' `union` singleton ex
+  | θ' ; x => fv_ss θ' `union` singleton x
+  end.
+
+Fixpoint ss_to_ctx (θ : subst_set) : ld_context := 
+  match θ with 
+  | nil => ld_ctx_nil
+  | θ' ; x => ld_ctx_cons (ss_to_ctx θ') x
+  | θ' ; ex : t => ss_to_ctx θ'
+  end.
+
+Inductive wf_ss : subst_set -> Prop :=
+  | wf_ss_nil : wf_ss nil
+  | wf_ss_tv : forall x θ,
+      wf_ss θ -> x `notin` dom θ ->
+      wf_ss (θ; x)
+  | wf_ss_ev : forall ex t Θ, 
+     wf_ss Θ -> 
+     ex `notin` dom Θ ->
+     ld_wf_type (ss_to_ctx Θ) t -> 
+     ld_mono_type t ->
+     wf_ss (Θ; ex : t)
+.
+
+Lemma wf_uniq : forall Θ,
+    wf_ss Θ -> uniq Θ.
+Proof.
+  induction 1; eauto.
+Qed.
+
+
+Lemma wf_mono : forall θ x t, 
+  wf_ss θ -> x : t ∈ θ -> ld_mono_type t.
+Proof.
+  intros.
+  induction H.
+  - inversion H0.
+  - inversion H0.
+    inversion H2.
+    auto.
+  - inversion H0.
+    + dependent destruction H4. auto.
+    + auto.
+Qed.
+
+Reserved Notation "θ ⫦ t ⇝ t'"
+  (at level 65, t at next level, no associativity).
+Inductive inst_type : subst_set -> la_type -> ld_type -> Prop := 
+  | inst_t_tvar : forall θ x, 
+      wf_ss θ -> 
+      θ ⫦ (la_t_tvar_f x) ⇝ (ld_t_var_f x)
+  | inst_t_evar : forall θ x tᵈ, 
+      wf_ss θ -> 
+      x : tᵈ ∈ θ -> 
+      θ ⫦ (la_t_evar x) ⇝ tᵈ
+  | inst_t_int : forall θ, 
+      wf_ss θ -> 
+      θ ⫦ la_t_int ⇝ ld_t_int
+  | inst_t_arrow : forall θ Aᵃ Bᵃ Aᵈ Bᵈ, 
+      θ ⫦ Aᵃ ⇝ Aᵈ -> 
+      θ ⫦ Bᵃ ⇝ Bᵈ ->
+      θ ⫦ (la_t_arrow Aᵃ Bᵃ) ⇝ (ld_t_arrow Aᵈ Bᵈ)
+  | inst_t_intersection : forall θ Aᵃ Bᵃ Aᵈ Bᵈ,
+      θ ⫦ Aᵃ ⇝ Aᵈ -> 
+      θ ⫦ Bᵃ ⇝ Bᵈ ->
+      θ ⫦ (la_t_intersection Aᵃ Bᵃ) ⇝ (ld_t_intersection Aᵈ Bᵈ)
+  | inst_t_union : forall θ Aᵃ Bᵃ Aᵈ Bᵈ,
+      θ ⫦ Aᵃ ⇝ Aᵈ -> 
+      θ ⫦ Bᵃ ⇝ Bᵈ ->
+      θ ⫦ (la_t_union Aᵃ Bᵃ) ⇝ (ld_t_union Aᵈ Bᵈ)
+  | inst_t_forall : forall θ L A' A,
+      (forall x, x `notin` L -> 
+        θ ⫦ (open_la_type_wrt_la_type A' (la_t_tvar_f x)) ⇝ (open_ld_type_wrt_ld_type A (ld_t_var_f x))) ->
+      θ ⫦ (la_t_forall A') ⇝ (ld_t_forall A)
+where "θ ⫦ t ⇝ t'" := (inst_type θ t t').
+
+Lemma inst_t_wf_ss : forall θ t t',
+  θ ⫦ t ⇝ t' -> wf_ss θ.
+Proof.
+  induction 1; pick fresh x'; eauto.
+Qed.
+
+
+Reserved Notation "θ ⫦ Γᵃ ⇝ Γᵈ ⫣ θ'"
+  (at level 65, Γᵃ at next level, Γᵈ at next level, no associativity).
+Inductive inst_worklist : subst_set -> la_worklist -> ld_worklist -> subst_set -> Prop := 
+  | inst_wl_nil : forall θ, 
+      wf_ss θ -> 
+      θ ⫦ la_wl_nil ⇝ ld_wl_nil ⫣ θ
+  | inst_wl_sub : forall θ θ' Γᵃ t1ᵃ t2ᵃ Γᵈ t1ᵈ t2ᵈ, 
+      θ ⫦ Γᵃ ⇝ Γᵈ ⫣ θ' -> 
+      θ' ⫦ t1ᵃ ⇝ t1ᵈ -> 
+      θ' ⫦ t2ᵃ ⇝ t2ᵈ -> 
+      θ ⫦ (la_wl_cons_w Γᵃ (la_w_sub t1ᵃ t2ᵃ)) ⇝ (ld_wl_cons_w Γᵈ (ld_w_sub t1ᵈ t2ᵈ)) ⫣ θ'
+  | inst_wl_tv : forall θ θ' x Γᵃ Γᵈ, 
+      θ ⫦ Γᵃ ⇝ Γᵈ ⫣ θ' -> 
+      θ ⫦ (la_wl_cons_tv Γᵃ x) ⇝ (ld_wl_cons_tv Γᵈ x) ⫣ (θ'; x)
+  | inst_wl_ev : forall θ θ' ex lbᵃ ubᵃ lbᵈ ubᵈ Γᵃ Γᵈ, 
+      θ ⫦ Γᵃ ⇝ Γᵈ ⫣ θ' -> 
+      θ ⫦ lbᵃ ⇝ lbᵈ ->
+      θ ⫦ ubᵃ ⇝ ubᵈ ->
+      θ ⫦ (la_wl_cons_ev Γᵃ lbᵃ ex ubᵃ) ⇝ (ld_wl_cons_w Γᵈ (ld_w_sub lbᵈ ubᵈ)) ⫣ (θ' ; ex : lbᵈ)
+where "θ ⫦ Γᵃ ⇝ Γᵈ ⫣ θ'" := (inst_worklist θ Γᵃ Γᵈ θ').
+
+
+Hint Constructors inst_type : transfer.
+Hint Constructors inst_worklist : transfer.
+
+
+Lemma fv_ss_ld_ctx_dom: forall θ x,
+  x `notin` fv_ss θ -> x `notin` ld_ctx_dom (ss_to_ctx θ).
+Proof.
+  induction θ; simpl; intros; auto.
+  - destruct a; destruct s.
+    + simpl in *. auto.
+    + auto.
+Qed.
+
+
+Lemma notin_wf_t_notin_ss: forall t θ x,
+  ss_to_ctx θ ⊢ t -> x `notin` fv_ss θ -> x `notin` fv_ld_type t.
+Proof.
+  induction t; intros.
+  - auto.
+  - simpl. dependent destruction H.
+    inst_cofinites_by (L `union` singleton x).
+    eapply ld_wf_type_fv with (x:=x) in H.
+    rewrite fv_ld_type_open_ld_type_wrt_ld_type_lower.
+    eauto. simpl. auto.
+    apply notin_add; auto.
+    apply fv_ss_ld_ctx_dom. auto.
+  - simpl. dependent destruction H; apply notin_union; eauto.
+  - simpl. dependent destruction H; apply notin_union; eauto.
+  - simpl. dependent destruction H; apply notin_union; eauto.
+  - auto.
+  - dependent destruction H; auto.
+    clear H.
+    induction θ; auto.
+    + inversion H0.
+    + destruct a. destruct s; simpl in *.
+      inversion H0; subst; auto.
+      auto.
+Qed.
+
+Lemma notin_ss_notin_inst : forall θ x ex t,
+    wf_ss θ ->
+    ex : t ∈ θ -> 
+    x `notin` fv_ss θ ->
+    x `notin` fv_ld_type t.
+Proof.
+  intro θ.
+  induction θ; intros.
+  - inversion H0.
+  - inversion H0. destruct a; destruct s.
+    + inversion H2.
+    + inversion H2. subst. inversion H. subst. 
+      simpl in H1. eapply notin_wf_t_notin_ss; eauto.
+    + eapply IHθ; eauto. inversion H; auto.
+      destruct a; destruct s; simpl in *. auto. auto.
+Qed.
+
+Lemma inst_t_lc : forall θ Aᵃ Aᵈ, 
+  θ ⫦ Aᵃ ⇝ Aᵈ -> 
+  lc_la_type Aᵃ /\ lc_ld_type Aᵈ.
+Proof.
+  intros.
+  induction H; try (split; destruct_conjs; auto; fail).
+  - split. auto. 
+    induction θ.
+    + inversion H0.
+    + destruct a. inversion H0.
+      * inversion H1. subst. inversion H.
+        subst. now apply ld_mono_is_ld_lc.
+      * inversion H. apply IHθ; auto. auto.
+  - split; inst_cofinites_by L.
+    + apply lc_la_t_forall_exists with (x1:=x). intuition.
+    + apply lc_ld_t_forall_exists with (x1:=x). intuition.
+Qed.
+
+
+Ltac inversion_eq :=
+  repeat
+    match goal with 
+        | H : ?a = ?b |-  _ => dependent destruction H
+      end.
+
+Lemma inst_A_det : forall θ Aᵃ A₁ᵈ,
+  uniq θ -> 
+  θ ⫦ Aᵃ ⇝ A₁ᵈ -> 
+  forall A₂ᵈ, θ ⫦ Aᵃ ⇝ A₂ᵈ -> 
+    A₁ᵈ = A₂ᵈ.
+Proof.
+  induction 2; (intros e₂ᵈ H2; dependent destruction H2; auto). 
+  - specialize (binds_unique _ _ _ _ _ H1 H3).
+    intros. specialize (H4 H). inversion_eq. auto.
+  - specialize (IHinst_type1 H _ H2_).
+    specialize (IHinst_type2 H _ H2_0).
+    subst. auto.
+  - inst_cofinites_by (L `union` L0 `union` (fv_ld_type A) `union` (fv_ld_type A0)).  
+    assert (A = A0).
+    + eapply open_ld_type_wrt_ld_type_inj with (x1:=x); auto.
+    + subst. auto. 
+Qed.
+
+
+Lemma not_in_dom_not_in_fv_ss: forall x θ,
+  x `notin` dom θ -> 
+  x `notin` fv_ss θ.
+Proof.
+  induction θ; auto.
+  destruct a. destruct s; simpl; 
+  intros; apply notin_union; auto.
+Qed.
+
+
+Lemma inst_e_rename : forall θ Aᵃ Aᵈ x x'
+  , θ ⫦ Aᵃ ⇝ Aᵈ 
+  -> x `notin` dom θ
+  -> θ ⫦ [`ᵃ x' /ᵃ x] Aᵃ ⇝ [`ᵈ x' /ᵈ x] Aᵈ.
+Proof with auto with transfer.
+  intros. induction H; simpl; auto...
+  - unfold eq_dec. destruct (EqDec_eq_of_X x0 x); auto...
+  - rewrite subst_ld_type_fresh_eq. auto...
+    eapply notin_ss_notin_inst; eauto.
+    now apply not_in_dom_not_in_fv_ss. 
+  - eapply inst_t_forall with (L := L `union` singleton x). intros.
+    rewrite_la_subst_open_var. rewrite_ld_subst_open_var. auto.
+Qed.
+
+
+Lemma inst_e_rev_subst' : forall tᵃ tᵈ x θ Aᵃ,
+  lc_la_type Aᵃ -> 
+  x `notin` (fx_la_type tᵃ `union` fv_ss θ) -> 
+  θ ⫦ tᵃ ⇝ tᵈ -> 
+  forall A'ᵈ, θ ⫦ [tᵃ /ᵃ x] Aᵃ ⇝ A'ᵈ
+    -> exists Aᵈ, [tᵈ /ᵈ x] Aᵈ = A'ᵈ /\ θ ⫦ Aᵃ ⇝ Aᵈ.
+Proof with auto with transfer.
+  intros * Hlc Hfv Hinstt.
+  induction Hlc; intros * HinstA; simpl in *.
+  - inversion HinstA. exists ld_t_int. simpl. split; auto...
+  - specialize (inst_t_lc _ _ _ Hinstt). intros.
+    dependent destruction HinstA.
+    inst_cofinites_by (L `union` singleton x `union` fv_ld_type tᵈ `union`  fv_ld_type A `union` dom θ `union` fx_la_type t). 
+    replace (`ᵃ x0) with ([tᵃ /ᵃ x] (`ᵃ x0)) in H1 by (apply subst_la_type_fresh_eq; auto).
+    rewrite <- subst_la_type_open_la_type_wrt_la_type in H1.
+    specialize (H0 _ _ H1).
+    destruct H0 as [A'ᵈ HinstA'ᵈ].
+    exists (ld_t_forall (close_ld_type_wrt_ld_type x0 A'ᵈ)). simpl.
+    rewrite subst_ld_type_close_ld_type_wrt_ld_type. 
+    + split.
+      * f_equal. destruct_conjs. apply ld_type_open_r_close_l; auto. 
+      * eapply inst_t_forall with (L:=L); intros.
+        rewrite (subst_la_type_intro x0) by auto.
+        rewrite (subst_ld_type_intro x0) by (apply close_ld_type_notin).
+        apply inst_e_rename; auto.
+        rewrite open_ld_type_wrt_ld_type_close_ld_type_wrt_ld_type. intuition.
+    + intuition. 
+    + auto.
+    + auto.
+    + intuition.
+  - dependent destruction HinstA.
+    specialize (IHHlc1 _ HinstA1). destruct IHHlc1 as [t₁ᵈ HinstA1inv].
+    specialize (IHHlc2 _ HinstA2). destruct IHHlc2 as [t₂ᵈ HinstA2inv].
+    exists (ld_t_arrow t₁ᵈ t₂ᵈ). destruct_conjs. split; simpl; subst; auto...
+  - exists (ld_t_var_f x5).
+    destruct (x5 == x).  
+    + subst. simpl. destruct (x == x).
+      * split.
+        -- assert (uniq θ) as Huniq by (apply wf_uniq; eapply inst_t_wf_ss; eauto).
+           specialize (inst_A_det _ _ _ Huniq Hinstt). intros.
+           specialize (H _ HinstA). auto.
+        -- constructor. eapply inst_t_wf_ss. eauto.
+      * contradiction.
+    + simpl. unfold eq_dec. destruct (EqDec_eq_of_X x5 x).
+      * contradiction.
+      * inversion HinstA; split; auto... 
+  - simpl in *. exists A'ᵈ. split.
+    + rewrite subst_ld_type_fresh_eq. auto.
+      inversion HinstA.
+      eapply notin_ss_notin_inst; eauto.
+    + auto.
+Qed.
+
+Lemma inst_wf : forall θ tᵃ tᵈ,
+  θ ⫦ tᵃ ⇝ tᵈ -> wf_ss θ.
+Proof.
+  intros. induction H; auto.
+  - inst_cofinites_by L. auto.
+Qed.
+
+Lemma inst_e_rev_subst : forall A'ᵈ θ tᵃ tᵈ x Aᵃ,
+  lc_la_type Aᵃ ->
+  x `notin` (fx_la_type tᵃ `union` fv_ss θ) -> 
+  θ ⫦ tᵃ ⇝ tᵈ → θ ⫦ [tᵃ /ᵃ x] Aᵃ ⇝ A'ᵈ ->
+  exists Aᵈ, [tᵈ /ᵈ x] Aᵈ = A'ᵈ ∧ θ ⫦ Aᵃ ⇝ Aᵈ.
+Proof.
+  intros.  
+  specialize (inst_e_rev_subst' _ _ _ _  _ H H0 H1 A'ᵈ).
+  intros.
+  specialize (H3 H2).
+  auto.
+Qed.
+
+Fixpoint ld_type_to_la_type (Aᵈ : ld_type) : la_type :=
+  match Aᵈ with 
+  | ld_t_int => la_t_int
+  | ld_t_forall A'ᵈ => la_t_forall (ld_type_to_la_type A'ᵈ)
+  | ld_t_arrow A₁ᵈ A₂ᵈ => la_t_arrow (ld_type_to_la_type A₁ᵈ) (ld_type_to_la_type A₂ᵈ)
+  | ld_t_var_b n => la_t_tvar_b n
+  | ld_t_var_f x => la_t_tvar_f x
+  end.
+
+Lemma ld_type_to_la_type_open_open_expr_wrt_expr_distr_rec : forall e1 e2 n,
+ld_type_to_la_type (open_ld_type_wrt_ld_type_rec n e2 e1) = open_la_type_wrt_la_type_rec n (ld_type_to_la_type e2) (ld_type_to_la_type e1).
+Proof.
+  intros e1.
+  induction e1; simpl; intros; auto.
+  - rewrite IHe1. auto.
+  - rewrite IHe1_1. rewrite IHe1_2. auto.
+  - destruct (lt_eq_lt_dec n n0).
+    + destruct s; simpl. auto.
+      auto.
+    + simpl. auto.
+Qed.
+
+Lemma ld_type_to_la_type_open_open_expr_wrt_expr_distr : forall e1 e2,
+  ld_type_to_la_type (open_ld_type_wrt_ld_type e1 e2) = open_la_type_wrt_la_type
+  (ld_type_to_la_type e1)(ld_type_to_la_type e2) .
+Proof.
+  intros.
+  unfold open_la_type_wrt_la_type.
+  unfold open_ld_type_wrt_ld_type.
+  rewrite ld_type_to_la_type_open_open_expr_wrt_expr_distr_rec.
+  auto.
+Qed.
+
+Lemma inst_ld_type_to_la_type: forall θ Aᵈ,
+  lc_ld_type Aᵈ ->
+  wf_ss θ ->
+  θ ⫦ ld_type_to_la_type Aᵈ ⇝ Aᵈ.
+Proof.
+  intros * Hlc.
+  induction Hlc; simpl; try (constructor; auto; fail).
+  - intros.
+    eapply inst_t_forall with (L:=empty).
+    intros.
+    specialize (H0 x H1).
+    rewrite ld_type_to_la_type_open_open_expr_wrt_expr_distr in H0.
+    simpl in *.
+    eauto.
+Qed.
+
+
+Lemma ld_type_to_la_type_open_rec_distr: forall t1ᵈ t2ᵈ n, 
+  ld_type_to_la_type (open_ld_type_wrt_ld_type_rec n t2ᵈ t1ᵈ) = open_la_type_wrt_la_type_rec n (ld_type_to_la_type t2ᵈ) (ld_type_to_la_type t1ᵈ).
+Proof.
+  intro t1ᵈ; induction t1ᵈ; intros; auto.
+  - simpl. rewrite IHt1ᵈ.
+    auto.
+  - simpl. rewrite IHt1ᵈ1. rewrite IHt1ᵈ2. auto.
+  - simpl. destruct (lt_eq_lt_dec n n0); simpl; auto.
+    + destruct s; auto.
+Qed.
+
+
+Lemma ld_type_to_la_type_open_distr: forall t1ᵈ t2ᵈ , 
+  ld_type_to_la_type (open_ld_type_wrt_ld_type t1ᵈ t2ᵈ ) = open_la_type_wrt_la_type (ld_type_to_la_type t1ᵈ) (ld_type_to_la_type t2ᵈ).
+Proof.
+  intros. unfold open_ld_type_wrt_ld_type. unfold open_la_type_wrt_la_type.
+  rewrite ld_type_to_la_type_open_rec_distr. auto.
+Qed.
+
+Lemma ld_type_to_la_type_open_var_distr: forall t1ᵈ x , 
+  ld_type_to_la_type (t1ᵈ ^ᵈ x) = (ld_type_to_la_type t1ᵈ) ^ᵃ x.
+Proof.
+  intros. 
+  replace (`ᵃ x) with (ld_type_to_la_type (`ᵈ x)) by auto.
+  rewrite ld_type_to_la_type_open_distr.
+  auto.
+Qed.
+
+
+Lemma ld_type_to_la_type_keeps_lc: forall tᵈ,
+  lc_ld_type tᵈ -> lc_la_type (ld_type_to_la_type tᵈ).
+Proof.
+  intros. induction H; simpl; auto.
+  - econstructor. intros. simpl in *. simpl.
+    rewrite <- ld_type_to_la_type_open_var_distr.
+    auto.
+Qed.
+
+Lemma inst_subst : forall θ x tᵈ Aᵃ Aᵈ, 
+  lc_la_type Aᵃ ->
+  x `notin` (fx_la_type Aᵃ)->
+  (θ; x : tᵈ) ⫦ Aᵃ ⇝ Aᵈ -> 
+  θ ⫦ [ld_type_to_la_type tᵈ /^ᵃ x] Aᵃ ⇝ Aᵈ.
+Proof.
+  intros * Hlc Hfv Hinstopen.
+  generalize dependent Aᵈ.
+  dependent induction Hlc; simpl in *; intros.
+  - inversion Hinstopen. econstructor.
+    inversion H. auto.
+  - dependent destruction Hinstopen.
+    eapply inst_t_forall with (L:=singleton x `union` fx_la_type t `union` fex_la_type t `union` L). intros.
+    + intros.
+      rewrite la_type_ex_subst_open_comm.
+      * eapply H0.
+        apply fx_la_type_open_la_type_notin; auto.
+        auto.
+      * inst_cofinites_with x0.
+        apply inst_wf in H1.
+        inversion H1.
+        apply ld_type_to_la_type_keeps_lc. apply ld_mono_is_ld_lc. auto.
+      * auto.
+  - dependent destruction Hinstopen.
+    econstructor; auto.
+  - destruct (x5 == x).
+    + subst.
+      apply notin_singleton_1 in Hfv. 
+      contradiction.
+    + dependent destruction Hinstopen.
+      constructor. inversion H. auto. 
+  - dependent destruction Hinstopen. 
+    destruct (ex5 == x). 
+    + subst.
+      apply binds_unique with (a:=sse_ev tᵈ) in H0. inversion H0. subst. inversion H.
+      * apply inst_ld_type_to_la_type; auto. 
+        apply ld_mono_is_ld_lc. auto.
+      * constructor; auto.
+      * apply wf_uniq. auto.
+    + inversion H0. 
+      * dependent destruction H1.
+        contradiction.
+      * econstructor; auto.      
+        dependent destruction H. auto.
+Qed.
+
+
+(* Lemma transfer_reorder: forall Γᵃ Γ'ᵈ θ' x t m Γ'ᵃ,
+  reorder Γᵃ x t m la_wl_nil Γ'ᵃ ->
+  inst_worklist nil Γ'ᵃ Γ'ᵈ θ' ->
+  exists Γᵈ θ, inst_worklist nil Γᵃ Γᵈ θ.
+Proof.
+  intros. 
+  generalize dependent θ'.
+  generalize dependent Γ'ᵈ.
+  induction H; intros.
+  - admit.
+  - admit.
+  - dependent destruction H1.
+    specialize (IHreorder Γᵈ θ' H1).
+    destruct IHreorder as [Γ'ᵈ [θ'']].  
+    exists (ld_wl_cons_tv Γ'ᵈ y), θ''.
+    constructor. auto.
+  - dependent destruction H1.
+    specialize (IHreorder _ _ H1).
+    destruct IHreorder as [Γ'ᵈ].
+    exists Γ'ᵈ.
+    econstructor; auto. admit.
+  - dependent destruction H1.
+    specialize (IHreorder _ _ H1).
+    destruct IHreorder as [Γ'ᵈ].
+    exists Γ'ᵈ.
+    econstructor; eauto. admit.
+  - dependent destruction H0.
+    admit.
+Admitted.
+
+Lemma transfer_reorder': forall Γᵃ Γᵈ θ x t m Γ'ᵃ,
+  reorder Γᵃ x t m la_wl_nil Γ'ᵃ ->
+  inst_worklist nil Γᵃ Γᵈ θ -> 
+  exists Γ'ᵈ θ', inst_worklist nil Γ'ᵃ Γ'ᵈ θ'.
+Proof.
+  intros. 
+  generalize dependent θ.
+  generalize dependent Γᵈ.
+  induction H; intros.
+  - exists Γᵈ, θ. admit.
+  - admit.
+  - dependent destruction H1.
+    specialize (IHreorder Γᵈ θ' H1).
+    destruct IHreorder as [Γ'ᵈ [θ'']].  
+    exists (ld_wl_cons_tv Γ'ᵈ y), θ''.
+    econstructor. auto.
+  - dependent destruction H1.
+    specialize (IHreorder _ _ H1).
+    destruct IHreorder as [Γ'ᵈ [θ'']].
+    exists Γ'ᵈ, (θ''; y : tᵈ).
+    econstructor; auto.
+    + admit.
+    + admit.
+  - dependent destruction H1.
+    specialize (IHreorder _ _ H1).
+    destruct IHreorder as [Γ'ᵈ [θ'']].
+    exists Γ'ᵈ, (θ''; y : tᵈ).
+    econstructor; eauto.
+    + admit.
+    + admit.
+  - dependent destruction H0.
+Admitted. *)
+
+
+Definition transfer (Γ : la_worklist) (Γ' : ld_worklist) : Prop :=
+  exists θ', inst_worklist nil Γ Γ' θ'.
